Flesh out local correctness

Tealeaves/Backends/Adapters/NamedToLN.v
@@ -14,6 +14,8 @@ From Tealeaves Require Import
 Import Subset.Notations.
 Import Classes.Categorical.DecoratedFunctorPoly.
 Import List.ListNotations.
+Import ContainerFunctor.Notations.
+Import Monoid.Notations.
 Import DecoratedContainerFunctor.Notations.
 
 #[local] Generalizable Variables W T U.
@@ -79,12 +81,31 @@ Section with_DTM.
 
   Context
     (T: Type -> Type -> Type)
-    `{Categorical.DecoratedFunctorPoly.DecoratedFunctorPoly T}.
+    `{Categorical.DecoratedTraversableFunctorPoly.DecoratedTraversableFunctorPoly T}.
 
   Import Kleisli.DecoratedFunctorPoly.
   Import CategoricalToKleisli.DecoratedFunctorPoly.
   Import CategoricalToKleisli.DecoratedFunctorPoly.DerivedOperations.
   Import CategoricalToKleisli.DecoratedFunctorPoly.DerivedInstances.
+  Import CategoricalToKleisli.DecoratedTraversableFunctorPoly.DerivedOperations.
+
+  Import DecoratedFunctorPoly.ToMono.
+  Import TraversableFunctor2.ToMono.
+  Import PolyToMono.Kleisli.DecoratedFunctor.ToMono1.
+
+  Import CategoricalToKleisli.TraversableFunctor.DerivedOperations.
+  Import CategoricalToKleisli.TraversableFunctor.DerivedInstances.
+
+  Import CategoricalToKleisli.DecoratedTraversableFunctor.DerivedOperations.
+  Import CategoricalToKleisli.DecoratedTraversableFunctor.DerivedInstances.
+
+  Existing Instance Theory.DecoratedTraversableFunctor.ToCtxset_Mapdt.
+  Existing Instance Theory.TraversableFunctor.ToSubset_Traverse.
+
+
+  Fail Import Categorical.DecoratedTraversableFunctorPoly.ToMono.
+
+  Context `{! DecoratedTraversableFunctor (list atom) (T atom)}. (* TODO Infer this *)
 
   (** ** Named to Locally Nameless *)
   (********************************************************************)
@@ -92,7 +113,7 @@ Section with_DTM.
     fun b =>
       match b with
       | Bound prefix var postfix =>
-          Bd (length prefix)
+          Bd (length postfix)
       | Unbound context var =>
           Fr var
       end.
@@ -110,42 +131,277 @@ Section with_DTM.
 
   (** ** Locally Nameless to Named *)
   (********************************************************************)
-  Definition INDEX_EXCEEDS_CONTEXT: nat := 1337.
+  (* crash hard, crash often *)
+  Definition PANIC_INDEX_EXCEEDS_CONTEXT: nat := 1337.
 
-  Fixpoint ix_new_name_core (avoid: list name) (n: nat): name :=
-    match n with
-    | 0 => fresh avoid
-    | S n' => fresh (avoid ++ [ix_new_name_core avoid n'])
+  (** ** <<to_name_from_history>> *)
+  (********************************************************************)
+  (** Perform one local binder renaming on a locally nameless binder occurrence, given
+      the history (the names assigned to binders higher in the tree) and the initial avoid set. *)
+  Definition to_name_from_history (top_conflicts: list name) (p: list name * unit): name :=
+    match p with
+    | (history, u) => fresh (top_conflicts ++ history)
+    end.
+
+
+  (** *** Rewriting Principles for <<to_name_from_history>> *)
+  (********************************************************************)
+  Lemma to_name_from_history_nil (top_conflicts: list name) (u: unit):
+    to_name_from_history top_conflicts (@nil atom, u) = fresh top_conflicts.
+  Proof.
+    cbn.
+    rewrite List.app_nil_r.
+    reflexivity.
+  Qed.
+
+  Lemma to_name_from_history_pair (top_conflicts: list name) (history: list atom) (u: unit):
+    to_name_from_history top_conflicts (history, u) = fresh (top_conflicts ++ history).
+  Proof.
+    reflexivity.
+  Qed.
+
+  Lemma to_name_from_history_preincr (top_conflicts: list name) (ctx: list atom):
+    to_name_from_history top_conflicts ⦿ ctx = to_name_from_history (top_conflicts ++ ctx).
+  Proof.
+    ext [w l].
+    unfold preincr, incr, compose.
+    rewrite to_name_from_history_pair.
+    unfold to_name_from_history.
+    fequal.
+    rewrite <- List.app_assoc.
+    reflexivity.
+  Qed.
+
+  (** *** Freshness for <<to_name_from_history>> *)
+  (********************************************************************)
+  Lemma to_name_from_history_fresh (top_conflicts: list name): forall p,
+      ~ (to_name_from_history top_conflicts p ∈ top_conflicts).
+  Proof.
+    intros.
+    unfold to_name_from_history.
+    destruct p.
+    specialize (fresh_not_in (top_conflicts ++ l)).
+    intros hyp contra.
+    apply hyp.
+    rewrite element_of_list_app.
+    now left.
+  Qed.
+
+  (** ** <<to_history_from_prefix>> *)
+  (********************************************************************)
+
+  (** Given a locally nameless binding context (a list of unit values, representing its length-many binders opened in
+      scope), convert the context into same-length list of names assigned to each binder, given a top-level avoid
+      set. *)
+  Definition to_history_from_prefix (top_conflicts: list name): list unit -> list name :=
+    fold_with_history (to_name_from_history top_conflicts).
+
+  Lemma to_history_from_prefix_preincr (top_conflicts: list name) (ctx: list atom):
+    fold_with_history (to_name_from_history top_conflicts ⦿ ctx) =
+      to_history_from_prefix (top_conflicts ++ ctx).
+  Proof.
+    ext l.
+    generalize dependent top_conflicts.
+    generalize dependent ctx.
+    induction l; intros.
+    - cbn.
+      reflexivity.
+    - rewrite fold_with_history_cons.
+      unfold to_history_from_prefix.
+      rewrite fold_with_history_cons.
+      fequal.
+      { unfold preincr, incr, compose.
+        change (ctx ● []) with (ctx ++ []).
+        rewrite List.app_nil_r.
+        cbn.
+        rewrite List.app_nil_r.
+        reflexivity.
+      }
+      { rewrite preincr_preincr.
+        rewrite IHl.
+        unfold to_history_from_prefix.
+        rewrite IHl.
+        change (?l1 ● ?l2) with (l1 ++ l2).
+        unfold to_history_from_prefix.
+        rewrite to_name_from_history_preincr.
+        rewrite List.app_assoc.
+        reflexivity.
+      }
+  Qed.
+
+  (* Tailored for use when the list is a nominal binding context decomposition *)
+  Corollary to_history_from_prefix_decompose (top_conflicts: list name) {l1 l2: list unit} {u: unit}:
+to_history_from_prefix top_conflicts (l1 ++ [u] ++ l2) =
+        to_history_from_prefix top_conflicts l1 ++
+          [to_name_from_history top_conflicts
+             (to_history_from_prefix top_conflicts l1, u)] ++
+          fold_with_history
+          (to_name_from_history top_conflicts ⦿
+             (to_history_from_prefix top_conflicts l1 ++
+                [to_name_from_history top_conflicts (to_history_from_prefix top_conflicts l1, u)])) l2.
+  Proof.
+    intros.
+    unfold to_history_from_prefix.
+    rewrite fold_with_history_decompose.
+    reflexivity.
+  Qed.
+
+
+  (** *** Rewriting rules *)
+  (********************************************************************)
+  Lemma to_history_from_prefix_nil (top_conflicts: list name):
+    to_history_from_prefix top_conflicts nil = nil.
+  Proof.
+    reflexivity.
+  Qed.
+
+  Lemma to_history_from_prefix_cons (top_conflicts: list name) (u: unit) (pre: list unit):
+    to_history_from_prefix top_conflicts (u :: pre) =
+      fresh top_conflicts :: to_history_from_prefix (top_conflicts ++ [fresh top_conflicts]) pre.
+  Proof.
+    unfold to_history_from_prefix.
+    rewrite fold_with_history_cons.
+    fequal.
+    - rewrite to_name_from_history_nil.
+      reflexivity.
+    - rewrite to_name_from_history_nil.
+      fequal.
+      ext [x y].
+      unfold preincr, incr, compose.
+      unfold_ops @Monoid_op_list.
+      unfold to_name_from_history.
+      rewrite List.app_assoc.
+      reflexivity.
+  Qed.
+
+  (** *** Freshness for <<to_history_from_prefix>> *)
+  (********************************************************************)
+  Lemma to_history_from_prefix_fresh (top_conflicts: list name): forall (prefix: list unit),
+    forall (a: name),
+      a ∈ top_conflicts ->
+      ~ a ∈ (to_history_from_prefix top_conflicts prefix).
+  Proof.
+    introv Hin.
+    unfold to_name_from_history.
+    enough (cut: forall (x: atom), x ∈ to_history_from_prefix top_conflicts prefix -> x <> a).
+    { intro contra.
+      specialize (cut a).
+      apply cut; auto.
+    }
+    apply fold_with_history_ind.
+    intros u h Hnotin.
+    specialize (to_name_from_history_fresh top_conflicts (h, u)).
+    intro Hfresh.
+    intro contra.
+    subst. contradiction.
+  Qed.
+
+  (** ** <<to_name_from_prefix>> *)
+  (********************************************************************)
+  Definition to_name_from_prefix (top_conflicts: list name): list unit * unit -> name :=
+    run_using_prefix (to_name_from_history top_conflicts).
+
+  (** *** Relation between <<to_history_from_prefix>> and <<to_name_from_prefix>> *)
+  (********************************************************************)
+  Lemma to_history_from_prefix_spec (top_conflicts: list name):
+    to_history_from_prefix top_conflicts =
+      mapdz (T := list) (to_name_from_prefix top_conflicts).
+  Proof.
+    unfold to_name_from_prefix.
+    rewrite run_using_prefix_spec.
+    reflexivity.
+  Qed.
+
+  (** *** Rewriting rules for <<to_name_from_prefix>> *)
+  (********************************************************************)
+  Lemma to_name_from_prefix_rw_nil (top_conflicts: list name): forall (u: unit),
+      to_name_from_prefix (top_conflicts) (nil, u) =
+        fresh top_conflicts.
+  Proof.
+    intros.
+    cbn.
+    rewrite List.app_nil_r.
+    reflexivity.
+  Qed.
+
+  Lemma to_name_from_prefix_rw_cons (top_conflicts: list name): forall (u: unit) (rest: list unit) (u': unit),
+      to_name_from_prefix (top_conflicts) (u :: rest, u') =
+        fresh
+    (top_conflicts ++
+       fresh top_conflicts ::
+       fold_with_history (preincr (to_name_from_history top_conflicts) [fresh top_conflicts]) rest).
+  Proof.
+    intros.
+    unfold to_name_from_prefix.
+    unfold run_using_prefix.
+    rewrite fold_with_history_cons.
+    unfold to_name_from_history at 1.
+    unfold to_name_from_history at 1.
+    rewrite List.app_nil_r.
+    unfold to_name_from_history at 2.
+    rewrite List.app_nil_r.
+    reflexivity.
+  Qed.
+
+  (** *** Freshness for <<to_name_from_prefix>> *)
+  (********************************************************************)
+  Lemma to_name_from_prefix_fresh (top_conflicts: list name) (prefix: list unit) (u: unit):
+    ~ to_name_from_prefix top_conflicts (prefix, u) ∈ top_conflicts.
+  Proof.
+    intros.
+    unfold to_name_from_prefix.
+    intro contra.
+    unfold run_using_prefix in contra.
+    specialize (to_name_from_history_fresh top_conflicts
+                  (fold_with_history (to_name_from_history top_conflicts) prefix, u)).
+    intro Hyp.
+    apply Hyp.
+    assumption.
+  Qed.
+
+  Fixpoint length_to_list_unit (length: nat): list unit :=
+    match length with
+    | 0 => nil
+    | S n => tt :: length_to_list_unit n
     end.
 
   (* Give a DB index (Bd N), define its new name *)
-  Definition ix_new_name (top_conflicts: list name) (ctx: list unit) (n: nat): nat :=
+  Definition LN_BD_to_binder_name (top_conflicts: list name) (ctx: list unit) (n: nat): atom :=
     if Nat.ltb n (length ctx)
-    then ix_new_name_core top_conflicts (n - length ctx)
-    else INDEX_EXCEEDS_CONTEXT.
+    then to_name_from_prefix top_conflicts (length_to_list_unit (length ctx - (n + 1)), tt)
+    else PANIC_INDEX_EXCEEDS_CONTEXT.
+
+  Lemma LN_BD_to_binder_name_fresh: forall avoid a ctx n,
+      length ctx > n ->
+      a ∈ avoid -> LN_BD_to_binder_name avoid ctx n <> a.
+  Proof.
+    introv Hlt Hin.
+    unfold LN_BD_to_binder_name.
+    apply PeanoNat.Nat.ltb_lt in Hlt.
+    rewrite Hlt.
+    intro contra.
+    subst.
+    apply to_name_from_prefix_fresh in Hin.
+    assumption.
+  Qed.
 
   Definition ln_to_name (top_conflicts: list name):
     list unit * LN -> name :=
     fun '(depth, v) =>
       match v with
       | Fr x => x
-      | Bd n => ix_new_name (top_conflicts) depth n
+      | Bd n => LN_BD_to_binder_name (top_conflicts) depth n
       end.
-
-  Definition ln_to_binder (top_conflicts: list name):
-    list unit * unit -> name :=
-    (fun '(ctx, _) => ix_new_name_core top_conflicts (length ctx)).
 
   Definition term_ln_to_nominal (conflicts: list name):
     T unit LN -> T name name :=
     mapdp (T := T)
-      (ln_to_binder conflicts)
+      (to_name_from_prefix conflicts)
       (ln_to_name conflicts).
 
 
   (** ** Roundtrip Specifications *)
   (********************************************************************)
-
   Definition roundtrip_Named `{Traverse (T unit)}:
     T name name -> T name name :=
     fun t => let t_ln := term_nominal_to_ln t
@@ -155,85 +411,140 @@ Section with_DTM.
     forall (t: T name name),
       roundtrip_Named t =
         mapdp
-          (kc_dz (ln_to_binder (free (mapdp (const tt) name_to_ln t))) (const tt))
-          (kc_dfunp (ln_to_name (free (mapdp (const tt) name_to_ln t))) (const tt) name_to_ln) t.
+          (kc_dz (to_name_from_prefix (free (term_nominal_to_ln t))) (const tt))
+          (kc_dfunp (ln_to_name (free (term_nominal_to_ln t))) (const tt) name_to_ln) t.
   Proof.
     intros.
     unfold roundtrip_Named.
-    unfold term_ln_to_nominal.
-    unfold term_nominal_to_ln.
     compose near t on left.
+    unfold term_nominal_to_ln at 2.
+    unfold term_ln_to_nominal at 1.
     rewrite kdfunp_mapdp2.
-    unfold kc_dfunp.
-    unfold kc_dz.
-    About kc_dz.
     reflexivity.
   Qed.
 
-  Import PolyToMono.Kleisli.DecoratedFunctor.ToMono1.
+  (** *** Lemmas about mapping (const tt) *)
+  (********************************************************************)
+  Lemma mapd_list_prefix_const: forall (A: Type) (w: list A),
+      mapdz (T := list) (const tt) w = map (F := list) (const tt) w.
+  Proof.
+    intros.
+    rewrite mapd_list_prefix_spec.
+    unfold compose.
+    induction w.
+    - reflexivity.
+    - cbn. fequal.
+      compose near (decorate_prefix_list w).
+      rewrite (fun_map_map).
+      rewrite <- IHw.
+      reflexivity.
+  Qed.
 
-  Lemma roundtrip_Named_spec2 `{Traverse (T unit)}:
+  Lemma cobind_Z_const: forall (A: Type),
+      cobind (A := A) (W := Z) (const tt) = map (F := Z) (const tt).
+  Proof.
+    introv.
+    ext [w a].
+    cbn.
+    rewrite mapd_list_prefix_const.
+    reflexivity.
+  Qed.
+
+  Lemma cobind_Z2_const: forall (A A' B: Type) (f: Z2 B A -> A'),
+      cobind_Z2 (B1 := B) (A1 := A) (const tt) f =
+        fun '(w, a) => (map (F := list) (const tt) w, f (w, a)).
+  Proof.
+    introv.
+    ext [w a].
+    cbn.
+    compose near w on left.
+    unfold_Z.
+    rewrite <- mapd_list_prefix_spec.
+    rewrite mapd_list_prefix_const.
+    reflexivity.
+  Qed.
+
+  (** *** Presented in terms of <<mapd>> composed with <<rename_binders>> *)
+  (********************************************************************)
+
+  (* Given a binding occurrence (pre, b) in a nominal term t,
+     return the new name of b after a Nominal~>LN~>Nominal roundtrip *)
+  Definition roundtrip_Binders (avoid: list atom): Z atom -> atom :=
+    to_name_from_prefix avoid ∘ map (const tt).
+
+  (* Given a variable occurrence (pre, v) in a nominal term t,
+     return the new name of v after a Nominal~>LN~>Nominal roundtrip *)
+  Definition roundtrip_Vars (avoid: list atom): Z2 atom atom -> atom :=
+    kc_dfunp (ln_to_name avoid) (const tt) name_to_ln.
+
+  Lemma roundtrip_Binders_spec (avoid: list atom):
+    mapdz (T := list) (roundtrip_Binders avoid) =
+      to_history_from_prefix avoid ∘ map (const tt).
+  Proof.
+    intros.
+    unfold roundtrip_Binders.
+    rewrite to_history_from_prefix_spec.
+    Set Keyed Unification.
+    rewrite (mapdz_map_list (A' := atom) (B := atom) (A := unit)).
+    Unset Keyed Unification.
+    reflexivity.
+  Qed.
+
+  Lemma roundtrip_Named_spec_decomposed:
     forall (t: T name name),
       roundtrip_Named t =
-        rename_binders
-          (kc_dz
-             (ln_to_binder (free (mapdp (const tt) name_to_ln t)))
-             (const tt))
-          (mapd (T := T name)
-             (kc_dfunp
-                (ln_to_name (free (mapdp (const tt) name_to_ln t)))
-                (const tt)
-                name_to_ln)
-             t).
+        let avoid := LN.free (term_nominal_to_ln t)
+        in rename_binders
+             (roundtrip_Binders avoid)
+             (mapd (T := T name) (roundtrip_Vars avoid) t).
   Proof.
     intros.
     rewrite roundtrip_Named_spec1.
+    unfold kc_dz.
+    rewrite cobind_Z_const.
     rewrite mapd_decompose.
     reflexivity.
   Qed.
 
-  Lemma term_nominal_to_ln_spec (conflicts: list name):
-    mapdp (T := T)
-      (ln_to_binder conflicts)
-      (ln_to_name conflicts) =
-      rename_binders (ln_to_binder conflicts) ∘ mapd (ln_to_name conflicts).
+  (** *** Roundtrip effect on context occurrences *)
+  (* if (ctx, a) ∈d t, then (roundtrip_Occ (free t) (ctx, a)) ∈d roundtrip t *)
+  (********************************************************************)
+  Definition roundtrip_Occ (avoid: list atom): list atom * atom -> list atom * atom :=
+    fun '(ctx, a) =>
+      (mapdz (roundtrip_Binders avoid) ctx, roundtrip_Vars avoid (ctx, a)).
+
+
+  Lemma roundtrip_Named_var_spec {avoid: list atom}:
+    (kc_dfunp
+       (ln_to_name (avoid))
+       (const tt)
+       name_to_ln) =
+      fun '(ctx, nm) =>
+        match binding_to_ln (get_binding ctx nm) with
+        | Fr x => x
+        | Bd n => LN_BD_to_binder_name avoid (map (const tt) ctx) n
+        end.
   Proof.
-    rewrite mapd_decompose.
+    ext [ctx nm].
+    unfold kc_dfunp.
+    unfold compose.
+    unfold cobind_Z2.
+    unfold compose.
+    unfold map_Z2.
+    cbn.
+    compose near ctx.
+    unfold_Z.
+    rewrite <- mapd_list_prefix_spec.
+    rewrite mapd_list_prefix_const.
     reflexivity.
   Qed.
 
-
-  Import DecoratedFunctorPoly.ToMono.
-  Import TraversableFunctor2.ToMono.
-  Import CategoricalToKleisli.TraversableFunctor.DerivedOperations.
-
-
-  Context
-    `{ToCtxset (list atom) (T atom)}
-     `{Traverse (T unit)}.
-
-  (*
-  Definition cobind_binders {B1 B2}:
-    forall (ρ: list B1 * B1 -> B2) (p: list B1 * B1), list B2 * B2 :=
-    fun ρ => cobind (W := Z) ρ.
-    *)
-
-  (*
-  Definition cobind_vars {B1 B2 V}:
-    forall (ρ: list B1 * B1 -> B2) (p: list B1 * V), list B2 * V :=
-    fun ρ => map_fst (mapd_list_prefix ρ).
-    *)
-
-  Definition rt_local_binders (avoid: list atom) (ctx: list atom): list atom :=
-    map (kc_dz (ln_to_binder avoid) (const tt)) (decorate_prefix_list ctx).
-
-  Definition rt_local_atom (avoid: list atom) (ctx: list atom) (a: atom): atom :=
-    ln_to_name avoid (map (const tt) ctx, name_to_ln (ctx, a)).
-
+  (** ** Deleting Binders *)
+  (********************************************************************)
   Lemma decorate_rename_binders {B1 B2 V}:
     forall (ρ: list B1 * B1 -> B2) (t: T B1 V),
       delete_binders (dec (T B2) (rename_binders ρ t)) =
-        delete_binders (map (F := T B1) (map_fst (mapd_list_prefix ρ)) (dec (T B1) t)).
+        delete_binders (map (F := T B1) (map_fst (mapdz (T := list) ρ)) (dec (T B1) t)).
   Proof.
     intros.
     unfold delete_binders.
@@ -284,7 +595,7 @@ Section with_DTM.
     forall (ρ: list B1 * B1 -> B2) (t: T B1 V),
       delete_binders (dec (T B2) (rename_binders ρ t)) =
         map (F := T unit)
-          (map_fst (mapd_list_prefix ρ))
+          (map_fst (mapdz (T := list) ρ))
           (delete_binders (dec (T B1) t)).
   Proof.
     intros.
@@ -294,96 +605,6 @@ Section with_DTM.
     rewrite fun2_map22_map21_commute.
     reflexivity.
   Qed.
-
-End with_DTM.
-
-(** * Relating Operations *)
-(**********************************************************************)
-Section with_DTM.
-
-  Context
-    (T: Type -> Type -> Type)
-      `{Categorical.DecoratedTraversableFunctorPoly.DecoratedTraversableFunctorPoly T}.
-
-  Import CategoricalToKleisli.DecoratedTraversableFunctor.DerivedOperations.
-  Import CategoricalToKleisli.DecoratedTraversableFunctorPoly.DerivedOperations.
-  Import Categorical.DecoratedFunctorPoly.ToMono.
-  Import Categorical.TraversableFunctor2.ToMono.
-  Import CategoricalToKleisli.TraversableFunctor.DerivedOperations.
-
-  Lemma normalize_foldMap {M} `{Monoid M} `(f: list name * name -> M): forall (t: T name name),
-      foldMapd f t = mapdtp (A2 := False) (G := const M) (T := T) (pure (F := const M) ∘ (const tt)) f t.
-  Proof.
-  Admitted.
-
-  Lemma FV_same_converson: forall (t: T name name),
-      FV (T name) t =
-        LN.free (term_nominal_to_ln T t).
-  Proof.
-    intros.
-    unfold FV.
-    unfold term_nominal_to_ln.
-    unfold free.
-    rewrite (foldMap_to_traverse1).
-    unfold_ops @Traverse_Categorical.
-    unfold_ops @Dist2_1.
-    unfold_ops @Map2_1.
-    reassociate -> on right.
-    rewrite (fun2_map_map).
-    unfold mapdp.
-    unfold DerivedOperations.Mapdp_Categorical.
-    change (?x ∘ id) with x; change (id ∘ ?x) with x.
-    unfold compose.
-    compose near (decp t).
-    rewrite (fun2_map_map).
-    rewrite normalize_foldMap.
-    unfold mapdtp.
-    unfold Mapdt_Categorical.
-    unfold TraversableFunctor.dist.
-    change (?f ○ ?g) with (f ∘ g).
-    unfold compose.
-    fequal.
-    fequal.
-    { ext [l v].
-        unfold compose.
-        unfold name_to_ln.
-        destruct (get_binding_spec l v) as [[Hbinding Hspec] | [pre [post [Hbinding [Hspec1 Hspec2]]]]].
-        - cbn.
-          rewrite Hbinding.
-          reflexivity.
-        - cbn.
-          rewrite Hbinding.
-          reflexivity.
-    }
-  Qed.
-
-End with_DTM.
-
-
-Section alpha_reasoning.
-
-  Context
-    (T: Type -> Type -> Type)
-      `{Categorical.DecoratedTraversableFunctorPoly.DecoratedTraversableFunctorPoly T}.
-
-  Import TraversableFunctor2.ToMono.
-  Import CategoricalToKleisli.TraversableFunctor.DerivedOperations.
-  Import CategoricalToKleisli.TraversableFunctor.DerivedInstances.
-  Import Theory.LiftRel.TraversableFunctor.
-
-  Import PolyToMono.Kleisli.DecoratedFunctor.
-  Import PolyToMono.Kleisli.DecoratedFunctor.ToMono1.
-
-  Import Categorical.DecoratedFunctorPoly.ToMono.
-  Import CategoricalToKleisli.DecoratedFunctorPoly.DerivedOperations.
-  Import CategoricalToKleisli.DecoratedFunctorPoly.DerivedInstances.
-
-  Import CategoricalToKleisli.DecoratedTraversableFunctor.DerivedOperations.
-  Import CategoricalToKleisli.DecoratedTraversableFunctor.DerivedInstances.
-
-  Fail Import Categorical.DecoratedTraversableFunctorPoly.ToMono.
-
-  Existing Instance Theory.TraversableFunctor.ToSubset_Traverse.
 
   Lemma in_del_binders {B A}: forall (t: T B A) (a: A),
       element_of a (delete_binders t) = element_of a t.
@@ -404,163 +625,249 @@ Section alpha_reasoning.
     reflexivity.
   Qed.
 
-  Import ContainerFunctor.Notations.
-
-  Definition rt_local (avoid: list atom): list atom * atom -> list atom * atom :=
-    fun '(ctx, a) =>
-    (map_fst (mapd_list_prefix (kc_dz (ln_to_binder avoid) (const tt)))
-       (cobind (kc_dfunp (ln_to_name avoid) (const tt) name_to_ln) (ctx, a))).
-
-  Lemma rt_local_spec (avoid: list atom): forall (p: list atom * atom),
-      rt_local avoid p = match p with
-                         | (ctx, a) => (rt_local_binders avoid ctx, rt_local_atom avoid ctx a)
-                         end.
+  (** ** Relating Free Variables During Translation *)
+  (********************************************************************)
+  Lemma normalize_foldMap {M} `{Monoid M} `(f: list name * name -> M): forall (t: T name name),
+      foldMapd f t = mapdtp (A2 := False) (G := const M) (T := T) (pure (F := const M) ∘ (const tt)) f t.
   Proof.
-    intros [ctx a].
-    unfold rt_local.
-    unfold kc_dz.
-    cbn.
-    destruct (get_binding_spec ctx a) as [[Case1 rest] | [prefix [postfix [Case2 [ctxspec Hnin]]]]].
-    { rewrite Case1.
-      unfold binding_to_ln.
-      fequal.
-      unfold rt_local_binders.
-      unfold kc_dz.
-      compose near ctx on right.
-      rewrite <- mapd_list_prefix_spec.
-      reflexivity.
-    }
-    { rewrite Case2.
-      repeat fequal.
-      - unfold rt_local_binders.
-        compose near ctx on right.
-        rewrite <- mapd_list_prefix_spec.
+  Admitted.
+
+  Lemma FV_preserved: forall (t: T name name),
+      FV (T name) t =
+        LN.free (term_nominal_to_ln t).
+  Proof.
+    intros.
+    unfold FV.
+    unfold term_nominal_to_ln.
+    unfold free.
+    rewrite (foldMap_to_traverse1).
+    unfold_ops @Traverse_Categorical.
+    unfold_ops @Dist2_1.
+    unfold_ops @Map2_1.
+    reassociate -> on right.
+    rewrite (fun2_map_map).
+    unfold mapdp.
+    unfold DerivedOperations.Mapdp_Categorical.
+    change (?x ∘ id) with x; change (id ∘ ?x) with x.
+    unfold compose.
+    compose near (decp t).
+    rewrite (fun2_map_map).
+    rewrite normalize_foldMap.
+    unfold mapdtp.
+    unfold DerivedOperations.Mapdt_Categorical.
+    unfold compose.
+    assert (cut: FV_loc = free_loc ∘ name_to_ln).
+    { ext [l v].
+      unfold compose.
+      unfold name_to_ln.
+      destruct (get_binding_spec l v) as [[Hbinding Hspec] | [pre [post [Hbinding [Hspec1 Hspec2]]]]].
+      - cbn.
+        rewrite Hbinding.
         reflexivity.
-      - clear.
-        induction ctx.
-        + reflexivity.
-        + cbn.
-          fequal.
-          compose near (decorate_prefix_list ctx).
-          rewrite (fun_map_map).
-          assert (cut: const tt ∘ incr (A := atom) [a] = const tt).
-          { now ext [? ?].
-          }
-          rewrite cut.
-          apply IHctx.
+      - cbn.
+        rewrite Hbinding.
+        reflexivity.
     }.
+    rewrite cut.
+    reflexivity.
   Qed.
 
-  Import Theory.DecoratedTraversableFunctor.
-  Existing Instance ToCtxset_Mapdt.
-
-  Lemma ln_to_binder_preincr: forall avoid a,
-      ln_to_binder avoid ∘ cobind (W := Z) (const tt) ∘ incr [a] =
-        ln_to_binder (avoid ++ [fresh avoid]) ∘ cobind (const tt).
+  (** ** Alpha Equivalence Local Reasoning *)
+  (********************************************************************)
+  Lemma to_name_from_prefix_preincr: forall avoid a,
+      to_name_from_prefix avoid ∘ cobind (W := Z) (const tt) ∘ incr [a] =
+        to_name_from_prefix (avoid ++ [fresh avoid]) ∘ cobind (const tt).
   Proof.
     intros.
     ext [ctx x].
     unfold compose.
-    unfold ln_to_binder.
+    unfold to_name_from_prefix.
   Abort.
 
-
-  Lemma rt_binders_rw: forall avoid l1 l2,
-      rt_local_binders avoid (l1 ++ l2) =
-        rt_local_binders avoid l1 ++ rt_local_binders (avoid ++ rt_local_binders avoid l1) (l1 ++ l2).
+  Lemma roundtrip_Occ_Unbound_spec1: forall (avoid: list atom) (ctx: list atom) (a: atom),
+      get_binding ctx a = Unbound ctx a ->
+      roundtrip_Occ avoid (ctx, a) = (mapdz (roundtrip_Binders avoid) ctx, a).
   Proof.
-    intros.
-    unfold rt_local_binders.
-    unfold kc_dz.
-    rewrite decorate_prefix_list_rw_app.
-    rewrite map_list_app.
-    compose near (decorate_prefix_list l2) on left.
-    rewrite map_list_app.
-    rewrite (fun_map_map).
-    fequal.
-    unfold cobind, Cobind_Z.
-    unfold mapd_Z.
-    induction l1.
-    - cbn.
-    unfold compose.
-    cbn.
-
-  Proof.
-
-  Lemma rt_binders_rw: forall avoid a ctx,
-      rt_local_binders avoid (a :: ctx)  =
-        fresh avoid :: rt_local_binders (avoid ++ [fresh avoid]) ctx.
-  Proof.
-    intros.
-    unfold rt_local_binders.
-    rewrite decorate_prefix_list_rw_cons.
-    rewrite map_list_cons.
-    fequal.
-    compose near (decorate_prefix_list ctx) on left.
-    rewrite fun_map_map.
-    fequal.
-    unfold kc_dz.
-    ext [w x].
-    unfold compose.
-    unfold incr.
-    unfold kc_dz.
-    unfold compose.
-    unfold monoid_op.
-    unfold Monoid_op_list.
-    change ([a] ++ w) with (a :: w).
-    rewrite cobind_Z_rw.
-    rewrite cobind_Z_rw.
-    rewrite  mapd_list_prefix_rw_cons.
-
+    introv Hyp.
     cbn.
     fequal.
+    rewrite Hyp.
+    cbn.
+    reflexivity.
+  Qed.
 
-  Lemma rt_correct_local:
-    forall (t: T name name) (avoid: list name)
-      (Havoidinit: forall (a: name), (a ∈ FV (T name) t -> a ∈ avoid)),
-      forall (ctx: list name) (a: name),
-        (ctx, a) ∈ (dec (T atom) t) ->
-        alpha_equiv_local (ctx, a)
-          (rt_local_binders avoid ctx, rt_local_atom avoid ctx a).
+  Lemma roundtrip_Occ_Bound_spec1: forall (avoid: list atom) (ctx: list atom) (a: atom) prefix a' postfix,
+      get_binding ctx a = Bound prefix a' postfix ->
+      roundtrip_Occ avoid (ctx, a) =
+        (mapdz (roundtrip_Binders avoid) ctx, roundtrip_Vars avoid (ctx, a)).
   Proof.
-    introv HavoidInit.
-    introv Helt.
-    destruct (get_binding_spec ctx a) as [[Case1 rest] | [prefix [postfix [Case2 [ctxspec Hnin]]]]].
-    {
-      unfold alpha_equiv_local.
-      rewrite Case1.
-      assert (HinFV: a ∈ FV (T name) t).
-      { assert (DecoratedTraversableFunctor (list atom) (T atom)).
-        { admit. }
-        apply (FV_lift_local (T atom) _ ctx); auto.
-      }
-      assert (HinAvoid: a ∈ avoid).
-      { apply HavoidInit; auto. }
+    introv Hyp.
+    clear Hyp.
+    unfold roundtrip_Occ.
+    rewrite roundtrip_Binders_spec.
+    reflexivity.
+  Qed.
 
-      Set Nested Proofs Allowed.
-  Lemma never_the_avoid_set: forall avoid ctx a,
+  Lemma roundtrip_Occ_Unbound_spec2: forall (avoid: list atom) (ctx: list atom) (a: atom),
       a ∈ avoid ->
-      ~ rt_local_atom avoid ctx a ∈ (rt_local_binders avoid ctx).
+      get_binding ctx a = Unbound ctx a ->
+      match roundtrip_Occ avoid (ctx, a) with
+      | (foo, x) =>
+          get_binding foo x = Unbound (mapdz (roundtrip_Binders avoid) ctx) a
+      end.
   Proof.
-    introv Hinavoid.
-    induction ctx.
-    - cbn. easy.
-    - unfold rt_local_atom.
-      unfold rt_local_binders.
-      rewrite map_list_cons.
-      rewrite map_list_cons_rw.
+    introv Hnin Hyp.
+    rewrite roundtrip_Occ_Unbound_spec1; auto.
+    destruct (get_binding_spec (mapdz (roundtrip_Binders avoid) ctx) a)
+      as [[Case1 rest] | [prefix [postfix [Case2 [ctxspec Hnin']]]]].
+    { rewrite Case1.
+      reflexivity. }
+    { assert (Hfresh: ~ a ∈ mapdz (roundtrip_Binders avoid) ctx).
+      { rewrite roundtrip_Binders_spec.
+        unfold compose at 1.
+        apply to_history_from_prefix_fresh.
+        assumption.
+      }
+      apply get_binding1 in Hfresh.
+      assumption.
+    }
+  Qed.
 
+  Lemma roundtrip_Vars_Bound_spec: forall (avoid: list atom) (ctx: list atom) (a: atom) prefix a' postfix,
+      get_binding ctx a = Bound prefix a' postfix ->
+      ctx = prefix ++ [a'] ++ postfix ->
+      a = a' ->
+      roundtrip_Vars avoid (ctx, a) =
+        to_name_from_history avoid (to_history_from_prefix avoid (map (const tt) prefix), tt).
+  Proof.
+    introv Hbinding Hctx Haeq.
+    unfold to_name_from_history.
+    unfold roundtrip_Vars.
+    unfold kc_dfunp.
+    rewrite cobind_Z2_const.
+    unfold compose at 1.
+    unfold name_to_ln.
+    rewrite Haeq in *; clear Haeq.
+    rewrite Hbinding.
+    unfold binding_to_ln.
+    unfold ln_to_name.
+    unfold LN_BD_to_binder_name.
+    rewrite map_preserve_length.
+    assert (HsafeIx: length postfix < length ctx).
+    { subst.
+      rewrite List.app_length.
+      rewrite List.app_length.
+      cbn.
+      lia.
+    }
+    rewrite <- PeanoNat.Nat.ltb_lt in HsafeIx.
+    rewrite HsafeIx.
+    unfold to_name_from_prefix.
+    unfold run_using_prefix.
+    unfold to_name_from_history.
+    fequal.
+    fequal.
+    unfold to_history_from_prefix.
+    fequal.
+    assert (Hineq: length ctx - (length postfix + 1) = length prefix).
+    { subst.
+      rewrite List.app_length.
+      rewrite List.app_length.
+      cbn.
+      lia.
+    }
+    rewrite Hineq.
+    { clear. induction prefix.
+      - reflexivity.
+      - cbn. now rewrite IHprefix. }
+  Qed.
+
+  Lemma roundtrip_Occ_Bound_spec2: forall (avoid: list atom) (ctx: list atom) (a: atom) prefix a' postfix,
+      get_binding ctx a = Bound prefix a' postfix ->
+      a = a' ->
+      ctx = prefix ++ [a'] ++ postfix ->
+      ~ a ∈ postfix ->
+      match roundtrip_Occ avoid (ctx, a) with
+      | (foo, x) =>
+          get_binding foo x =
+            let NewPrefix := to_history_from_prefix avoid (map (const tt) prefix)
+            in let NewVar := to_name_from_history avoid (NewPrefix, tt)
+               in let NewPost := to_history_from_prefix (avoid ++ NewPrefix ++ [NewVar]) (map (const tt) postfix)
+                  in Bound NewPrefix NewVar NewPost
+      end.
+  Proof.
+    introv Hyp Haeq Hctxeq Hnin.
+    unfold roundtrip_Occ.
+    rewrite roundtrip_Binders_spec.
+    unfold compose at 1.
+    remember (to_history_from_prefix avoid (map (const tt) ctx)) as NewContext.
+    remember (roundtrip_Vars avoid (ctx, a)) as NewVar'.
+    rewrite Hctxeq in HeqNewContext.
+    rewrite map_list_app in HeqNewContext.
+    rewrite map_list_app in HeqNewContext.
+    rewrite map_list_one in HeqNewContext.
+    change (const tt a') with tt in HeqNewContext.
+    rewrite (to_history_from_prefix_decompose avoid) in HeqNewContext.
+
+    remember (to_history_from_prefix avoid (map (const tt) prefix)) as NewPrefix.
+    remember (to_name_from_history avoid (NewPrefix, tt)) as NewVar.
+    rewrite (roundtrip_Vars_Bound_spec avoid ctx a prefix a' postfix Hyp Hctxeq Haeq) in HeqNewVar'.
+    assert (NewVar = NewVar').
+    { subst. reflexivity. }
+    rewrite <- H3 in *; clear H3.
+    rewrite to_name_from_history_preincr in HeqNewContext.
+    remember (fold_with_history (to_name_from_history avoid ⦿ (NewPrefix ++ [NewVar]))
+                (map (const tt) postfix)) as NewPostFix.
+    rewrite to_name_from_history_preincr in HeqNewPostFix.
+    unfold to_history_from_prefix.
+    rewrite <- HeqNewPostFix.
+    assert (Hnin': ~ NewVar ∈ NewPostFix).
+    { rewrite HeqNewPostFix.
       admit.
     }
+    rewrite HeqNewContext.
+    rewrite <- HeqNewPostFix.
+    admit.
+  Admitted.
+
+  Lemma rt_correct_local2:
+    forall (t: T name name) (avoid: list name)
+      (Havoidinit: forall (a: name), (a ∈ FV (T name) t -> a ∈ avoid)),
+    forall (ctx: list name) (a: name),
+      (ctx, a) ∈ (dec (T atom) t) ->
+      alpha_equiv_local (ctx, a) (roundtrip_Occ avoid (ctx, a)).
+  Proof.
+    introv HFV.
+    introv Hin.
+    unfold alpha_equiv_local.
+    destruct (get_binding_spec ctx a) as [[Case1 rest] | [prefix [postfix [Case2 [ctxspec Hnin]]]]].
+    { rewrite Case1.
+      assert (Havoid: a ∈ avoid).
+      { apply HFV.
+        apply (FV_lift_local (T atom) _ ctx); auto.
+      }
+      specialize (roundtrip_Occ_Unbound_spec2 avoid ctx a Havoid Case1).
+      intro X.
+      destruct (roundtrip_Occ avoid (ctx, a)).
+      rewrite X. destruct_eq_args a a.
+    }
     {
+      rewrite Case2.
+      apply (roundtrip_Occ_Bound_spec2 avoid) in Case2; auto.
+      destruct (roundtrip_Occ avoid (ctx, a)).
+      rewrite Case2.
+      cbn.
+      cbn.
+      admit.
     }
   Admitted.
 
   Lemma rt_correct_local1:  forall (t: T name name),
-    Forall
-    (fun a : list atom * atom =>
-     (precompose (cobind (kc_dfunp (ln_to_name (free (mapdp (const tt) name_to_ln t))) (const tt) name_to_ln))
-      ∘ (precompose (cobind_vars (kc_dz (ln_to_binder (free (mapdp (const tt) name_to_ln t))) (const tt)))
+    TraversableFunctor.Forall
+    (fun a: list atom * atom =>
+     (precompose (cobind (kc_dfunp (ln_to_name (free (term_nominal_to_ln t))) (const tt) name_to_ln))
+        ∘ (precompose (map_fst (mapd_list_prefix
+                                  (kc_dz (to_name_from_prefix (free (term_nominal_to_ln t))) (const tt))))
            ∘ alpha_equiv_local)) a a) (delete_binders (dec (T atom) t)).
   Proof.
     intros t.
@@ -568,22 +875,19 @@ Section alpha_reasoning.
     intros [ctx a].
     rewrite in_del_binders.
     unfold compose, precompose.
-    intros.
-    pose (rt_local_spec ((free (mapdp (const tt) name_to_ln t))) (ctx, a)).
-    unfold rt_local in e.
-    rewrite e.
-    eapply rt_correct_local; try eassumption.
-    { intro x.
-      rewrite (FV_same_converson T).
+    intro Hin.
+    apply (rt_correct_local2 t).
+    { rewrite (FV_preserved T t).
       easy.
     }
+    assumption.
   Qed.
 
   Theorem roundtrip_correct: forall (t: T name name),
       polymorphic_alpha T t (roundtrip_Named T t).
   Proof.
     intros.
-    rewrite (roundtrip_Named_spec2 T).
+    rewrite (roundtrip_Named_spec_decomposed T).
     unfold polymorphic_alpha.
     unfold lift_relation_ctx_poly.
     rewrite (decorate_rename_binders2 T).
@@ -597,4 +901,4 @@ Section alpha_reasoning.
 
   Print Assumptions roundtrip_correct.
 
-End alpha_reasoning.
+End with_DTM.
