Tealeaves/Backends/Named/Common.v
@@ -15,9 +15,8 @@ Import ContainerFunctor.Notations.
 
 Open Scope list_scope.
 
-(** * General operations on lists *)
+(** * The <<fold_with_history>> Operation *)
 (**********************************************************************)
-
 (* Fold over a list of A's where each A has the prefix of the list so far *)
 Fixpoint fold_with_history {A B: Type}
   (f: list B * A -> B)
@@ -28,8 +27,9 @@ Fixpoint fold_with_history {A B: Type}
       f ([], a) :: fold_with_history (f ⦿ [f ([], a)]) rest
   end.
 
+(** ** Rewriting rules for <<fold_with_history>> *)
+(**********************************************************************)
 Section rw.
-
 
   Context {A B: Type}.
 
@@ -79,7 +79,166 @@ Section rw.
       reflexivity.
   Qed.
 
+  (* Tailored for use when the list is a nominal binding context decomposition *)
+  Lemma fold_with_history_decompose {l1 l2: list A} {a: A}:
+    forall (f: list B * A -> B),
+      fold_with_history f (l1 ++ [a] ++ l2) =
+        fold_with_history f l1 ++
+          [f (fold_with_history f l1, a)] ++
+          fold_with_history (f ⦿ (fold_with_history f l1 ++ [f (fold_with_history f l1, a)])) l2.
+  Proof.
+    intros.
+    rewrite fold_with_history_app.
+    rewrite fold_with_history_app.
+    rewrite fold_with_history_one.
+    rewrite preincr_preincr.
+    unfold preincr, incr, compose.
+    unfold_ops @Monoid_op_list.
+    rewrite List.app_nil_r.
+    reflexivity.
+  Qed.
+
 End rw.
+
+(** ** An Induction Rule for <<fold_with_history>> *)
+(**********************************************************************)
+Section induction.
+
+  Import Theory.TraversableFunctor.
+
+  Context
+    {A B: Type}
+    {f: list B * A -> B}
+    (P: B -> Prop).
+
+  Section Forall.
+
+    Context
+      (Hbase: forall (a: A), P (f (nil, a)))
+      (Hstep: forall (a: A) (h: list B),
+      Forall P h -> P (f (h, a))).
+
+    Lemma fold_with_history_ind_Forall: forall (l: list A),
+        Forall P (fold_with_history f l).
+    Proof.
+      intro l.
+      induction l as [| a rest IHrest] using List.rev_ind.
+      - reflexivity.
+      - rewrite fold_with_history_app.
+        rewrite TraversableFunctor.forall_iff.
+        rewrite TraversableFunctor.forall_iff in IHrest.
+        intro b.
+        rewrite element_of_list_app.
+        intros [Case1| Case2].
+        + auto.
+        +rewrite fold_with_history_one in Case2.
+         rewrite element_of_list_one in Case2.
+         subst.
+         apply Hstep.
+         change (@nil B) with (Ƶ: list B).
+         rewrite monoid_id_l.
+         rewrite TraversableFunctor.forall_iff.
+         assumption.
+    Qed.
+
+  End Forall.
+
+  Section elementwise.
+
+    Context
+      (Hbase: forall (a: A), P (f (nil, a)))
+      (Hstep: forall (a: A) (h: list B),
+        (forall (b: B), b ∈ h -> P b) -> P (f (h, a))).
+
+    Lemma fold_with_history_ind: forall (l: list A),
+        forall (b: B), b ∈ fold_with_history f l -> P b.
+    Proof.
+      intro l.
+      rewrite <- TraversableFunctor.forall_iff.
+      apply fold_with_history_ind_Forall.
+      intros; apply Hstep.
+      rewrite TraversableFunctor.forall_iff in H.
+      assumption.
+    Qed.
+
+  End elementwise.
+
+End induction.
+
+(** ** Relating History to the Prefix: <<map_with_history>> *)
+(**********************************************************************)
+Section relate_history_prefix.
+
+  Context {A B: Type} (f: list B * A -> B).
+
+  Definition run_using_prefix: list A * A -> B :=
+    fun '(prefix, a) => f (fold_with_history f prefix, a).
+
+  Lemma run_using_prefix_app_spec: forall (l: list A) (a: A),
+      fold_with_history f (l ++ [a]) =
+        fold_with_history f l ++ [run_using_prefix (l, a)].
+  Proof.
+    intros.
+    rewrite fold_with_history_app.
+    fequal.
+    rewrite fold_with_history_one.
+    unfold preincr, incr, compose.
+    change (@nil B) with (Ƶ: list B) at 1.
+    rewrite monoid_id_l.
+    fequal.
+  Qed.
+
+  Lemma run_using_prefix_nil: forall (a: A),
+    run_using_prefix (nil, a) = f (nil, a).
+  Proof.
+    reflexivity.
+  Qed.
+
+  Lemma run_using_prefix_cons {a l x}:
+    run_using_prefix (a :: l, x) =
+      f (f ([], a) :: fold_with_history (f ⦿ [f ([], a)]) l, x).
+  Proof.
+    reflexivity.
+  Qed.
+
+  Lemma run_using_prefix_app {l1 l2 x}:
+    run_using_prefix (l1 ++ l2, x) =
+      f (fold_with_history f l1 ++ fold_with_history (f ⦿ fold_with_history f l1) l2, x).
+  Proof.
+    cbn.
+    rewrite fold_with_history_app.
+    reflexivity.
+  Qed.
+
+  Lemma run_using_prefix_one {a x}:
+    run_using_prefix ([a], x) =
+      f ([f ([], a)], x).
+  Proof.
+    cbn.
+    reflexivity.
+  Qed.
+
+End relate_history_prefix.
+
+Lemma run_using_prefix_spec {A B: Type} (f: list B * A -> B):
+  mapd_list_prefix (run_using_prefix f) =
+    fold_with_history f.
+Proof.
+  ext l.
+  generalize dependent f.
+  induction l; intros.
+  - cbn.
+    reflexivity.
+  - rewrite mapd_list_prefix_rw_cons.
+    rewrite fold_with_history_cons.
+    rewrite run_using_prefix_nil.
+    rewrite <- IHl.
+    fequal.
+    fequal.
+    ext [w a'].
+    cbn.
+    reflexivity.
+Qed.
 
 
 (** * Folding with context AND history *)
@@ -420,6 +579,123 @@ Section rw.
       autorewrite with tea_list. tauto.
   Qed.
 
+
+  Lemma list_app_one_inv {A}:
+    forall (prefix prefix': list A) (a a': A),
+      prefix ++ [a] = prefix' ++ [a'] ->
+      prefix = prefix' /\ a = a'.
+  Proof.
+    intros.
+    split.
+    eapply inv_app_eq_rl.
+    2: eassumption.
+    reflexivity.
+    enough (ListEq: [a] = [a']) by now inversion ListEq.
+    eapply inv_app_eq_rr; eauto.
+  Qed.
+
+  Lemma list_occ_spec {A}:
+    forall (prefix prefix' postfix: list A) (a a': A),
+      prefix ++ [a] = prefix' ++ [a'] ++ postfix ->
+        (prefix = prefix' /\ a = a' /\ postfix = []) \/ a ∈ postfix.
+  Proof.
+    intros.
+    { intros.
+      generalize dependent prefix.
+      generalize dependent prefix'.
+      generalize dependent a.
+      induction postfix using List.rev_ind; intros.
+      + rewrite List.app_nil_r in H.
+        apply list_app_one_inv in H.
+        left. tauto.
+      + right.
+        assert (a = x).
+        { do 2 rewrite List.app_assoc in H.
+          apply list_app_one_inv in H.
+          tauto.
+        }
+        subst.
+        rewrite element_of_list_app.
+        rewrite element_of_list_one.
+        now right.
+    }
+  Qed.
+
+
+  Lemma list_occ_lemma {A}:
+    forall (prefix prefix' postfix: list A) (a: A),
+      prefix ++ [a] = prefix' ++ [a] ++ postfix ->
+      (prefix = prefix' /\ postfix = []) \/ a ∈ postfix.
+  Proof.
+    intros.
+    apply list_occ_spec in H.
+    tauto.
+  Qed.
+
+  Lemma list_occ_lemma2 {A}:
+    forall (prefix prefix' postfix postfix' : list A) (v a: A),
+      v <> a ->
+      prefix ++ [v] ++ a :: postfix = prefix' ++ [v] ++ postfix' ->
+      exists postfix'', postfix' = a :: postfix''.
+  Proof.
+    intros.
+    induction postfix.
+    - exists (@nil A).
+      induction postfix'.
+      + specialize (list_occ_lemma prefix prefix' (@nil A) v).
+        intro.
+  Abort.
+
+  Lemma list_binding_inversion_prefix {A}:
+    forall (prefix postfix prefix' postfix': list A) (v: A)
+      (Hnin : ~ v ∈ postfix)
+      (Hnin': ~ v ∈ postfix'),
+      prefix ++ [v] ++ postfix = prefix' ++ [v] ++ postfix' ->
+      prefix = prefix' /\ postfix = postfix'.
+  Proof.
+    intros.
+    generalize dependent prefix.
+    generalize dependent prefix'.
+    generalize dependent v.
+    induction postfix; intros.
+    - rewrite List.app_nil_r in H.
+      specialize (list_occ_lemma _ _ _ v H).
+      destruct 1 as [[Hyp1 Hyp2] | Hyp3].
+      + subst. split; auto.
+      + contradiction.
+  Abort.
+
+
+
+  Lemma list_binding_inversion {A}:
+    forall (prefix postfix prefix' postfix': list A) (v: A)
+      (Hnin : ~ v ∈ postfix)
+      (Hnin': ~ v ∈ postfix'),
+      prefix ++ [v] ++ postfix = prefix' ++ [v] ++ postfix' ->
+      prefix = prefix' /\ postfix = postfix'.
+  Proof.
+    intros.
+  Admitted.
+
+
+  Lemma get_binding2: forall prefix v postfix ctx,
+      ctx = prefix ++ [v] ++ postfix ->
+      ~ (v ∈ postfix) ->
+      get_binding ctx v = Bound prefix v postfix.
+  Proof.
+    introv Heq Hnin. subst.
+    destruct (get_binding_spec (prefix ++ [v] ++ postfix) v)
+      as [[Case1 rest] | [prefix' [postfix' [Case2 [ctxspec Hnin']]]]].
+    - false. apply rest.
+      rewrite element_of_list_app.
+      rewrite element_of_list_app.
+      rewrite element_of_list_one.
+      tauto.
+    - rewrite Case2.
+      apply list_binding_inversion in ctxspec; auto.
+      destruct ctxspec; subst. reflexivity.
+  Qed.
+
 End rw.
 
 
@@ -432,79 +708,6 @@ Section rw.
   Compute get_binding l 3. (* Bound [1; 3; 4] 3 [2] *)
 
 End rw.
-
-
-
-(*
-  Lemma get_binding_rec_unbound1: forall l1 l2 a,
-  get_binding_rec_unbound l1 [a] l2 = Unbound (l1 + l) ->
-  get_binding_rec_unbound [a] l2 = Unbound (l1 + l) ->
-  get_binding_rec_unbound v [a] l
- *)
-
-
-(*
-
-  Fixpoint get_binding_rec (discarded: list name)  (l: list name) (looking_for: name): Binding :=
-  match l with
-  | nil => Unbound discarded
-  | cons y ys =>
-  if looking_for == y
-  then Bound discarded y ys
-  else get_binding_rec (discarded ++ [y]) ys looking_for
-  end.
-
-  Fixpoint get_binding_rec (discarded: list name)  (l: list name) (looking_for: name): Binding :=
-  match l with
-  | nil => Unbound discarded
-  | cons y ys =>
-  if looking_for == y
-  then Bound discarded y ys
-  else get_binding_rec (discarded ++ [y]) ys looking_for
-  end.
-
-
-  Definition get_binding: list name -> name -> Binding :=
-  get_binding_rec [].
-
-
-
-  Lemma get_binding_spec: forall (disc: list name) (l: list name) (v: name),
-  {get_binding_rec disc l v = Unbound (disc ++ l) /\ ~ v ∈ l} +
-  {exists pre post, get_binding_rec disc l v = Bound (disc ++ pre) v post  /\ l = pre ++ [v] ++ post /\ ~ v ∈ post}.
-  Proof.
-  intros.
-  induction l.
-  - cbn. left.
-  rewrite List.app_nil_r; split; auto.
-  - (* Lookup v in (a :: l) after discarding (disc). *)
-  cbn.
-  destruct_eq_args v a.
-  + right. destruct (IHl).
-  * exists (@nil name). exists l.
-  rewrite List.app_nil_r.
-  rewrite List.app_nil_l.
-  split. firstorder.
-  firstorder.
-  * destruct e as [pre [post [IH1 [IH2 IH3]]]].
-  exists (@nil name) post.
-  rewrite List.app_nil_r.
-  rewrite List.app_nil_l.
-  split; auto.
-  split; auto.
-  firstorder.
-
-  induction l.
-  { exists (@nil name) (@nil name).
-  rewrite List.app_nil_r.
-  rewrite List.app_nil_l.
-  split; auto.
-  }
-  { destruct
-  +
-
-  .
- *)
 
 Section examples.
 
